Prove gcm_blocks_stdcall wrapper

vale/code/arch/x64/interop/GCMencryptOpt_stdcalls.fsti
@@ -6,12 +6,17 @@ module B = LowStar.Buffer
 module HS = FStar.HyperStack
 module DV = LowStar.BufferView.Down
 module UV = LowStar.BufferView.Up
+open Vale.AsLowStar.MemoryHelpers
 open FStar.Mul
 open Words_s
 open Words.Seq_s
+open Types_s
 open GCM_helpers
 open AES_s
 open GCM_s
+open GHash_s
+open GCTR_s
+open GCTR
 open Interop.Base
 
 let uint8_p = B.buffer UInt8.t
@@ -28,6 +33,25 @@ let length_aux (b:uint8_p) : Lemma
 let length_aux2 (b:uint8_p) : Lemma
   (requires B.length b = 240)
   (ensures DV.length (get_downview b) % 16 = 0) = 
+    let db = get_downview b in
+    DV.length_eq db
+
+let length_aux3 (b:uint8_p) (n:nat) : Lemma
+  (requires B.length b = 16 * n)
+  (ensures DV.length (get_downview b) % 16 = 0) =
+    let db = get_downview b in
+    DV.length_eq db;
+    FStar.Math.Lemmas.cancel_mul_mod n 16
+
+let length_aux4 (b:uint8_p) : Lemma
+  (requires B.length b = 16)
+  (ensures DV.length (get_downview b) % 16 = 0) =
+    let db = get_downview b in
+    DV.length_eq db
+
+let length_aux5 (b:uint8_p) : Lemma
+  (requires B.length b = 160)
+  (ensures DV.length (get_downview b) % 16 = 0) =
     let db = get_downview b in
     DV.length_eq db
 
@@ -137,5 +161,77 @@ val gcm128_encrypt:
       Seq.equal (UV.as_seq h0 ub) (key_to_round_keys_LE AES_128 (Ghost.reveal key)))
     )
     (ensures fun h0 _ h1 ->
-      True
+      B.modifies (B.loc_union (B.loc_buffer tag_b)
+                  (B.loc_union (B.loc_buffer iv_b)
+                  (B.loc_union (B.loc_buffer scratch_b)
+                  (B.loc_union (B.loc_buffer out128x6_b)
+                  (B.loc_union (B.loc_buffer out128_b)
+                  (B.loc_buffer inout_b)))))) h0 h1 /\
+      (8 * (UInt64.v plain_num) < pow2_32 /\
+       8 * (UInt64.v auth_bytes) < pow2_32 /\ (
+       let in128x6_d = get_downview in128x6_b in
+       length_aux3 in128x6_b (UInt64.v len128x6);
+       let in128x6_u = UV.mk_buffer in128x6_d Views.up_view128 in
+       let in128_d = get_downview in128_b in
+       length_aux3 in128_b (UInt64.v len128_num);
+       let in128_u = UV.mk_buffer in128_d Views.up_view128 in
+       let inout_d = get_downview inout_b in
+       length_aux3 inout_b 1;      
+       let inout_u = UV.mk_buffer inout_d Views.up_view128 in       
+       let out128x6_d = get_downview out128x6_b in
+       length_aux3 out128x6_b (UInt64.v len128x6);
+       let out128x6_u = UV.mk_buffer out128x6_d Views.up_view128 in
+       let out128_d = get_downview out128_b in
+       length_aux3 out128_b (UInt64.v len128_num);
+       let out128_u = UV.mk_buffer out128_d Views.up_view128 in       
+       length_aux4 iv_b;
+       DV.length_eq (get_downview iv_b);
+       let iv_LE = low_buffer_read TUInt8 TUInt128 h0 iv_b 0 in
+       let iv_BE = reverse_bytes_quad32 iv_LE in
+       let ctr_BE_1 = Mkfour 1 iv_BE.lo1 iv_BE.hi2 iv_BE.hi3 in
+       let ctr_BE_2 = Mkfour 2 iv_BE.lo1 iv_BE.hi2 iv_BE.hi3 in
+       let plain_in =
+         if (UInt64.v plain_num > (UInt64.v len128x6 + UInt64.v len128_num) * 128/8) then
+           Seq.append (Seq.append (UV.as_seq h0 in128x6_u) (UV.as_seq h0 in128_u))
+                      (UV.as_seq h0 inout_u)
+         else Seq.append (UV.as_seq h0 in128x6_u) (UV.as_seq h0 in128_u)
+       in let cipher_out =
+         if (UInt64.v plain_num > (UInt64.v len128x6 + UInt64.v len128_num) * 128/8) then
+           Seq.append (Seq.append (UV.as_seq h1 out128x6_u) (UV.as_seq h1 out128_u))
+                      (UV.as_seq h1 inout_u)
+         else Seq.append (UV.as_seq h1 out128x6_u) (UV.as_seq h1 out128_u)
+       in gctr_partial AES_128 (UInt64.v len128x6 + UInt64.v len128_num + 1) plain_in cipher_out (Ghost.reveal key) ctr_BE_2 /\ (
+       DV.length_eq (get_downview hkeys_b);
+       let h = reverse_bytes_quad32 (low_buffer_read TUInt8 TUInt128 h1 hkeys_b 0) in
+       let length_quad = reverse_bytes_quad32 (Mkfour (8 * UInt64.v plain_num) 0 (8 * UInt64.v auth_bytes) 0) in
+       let auth_d = get_downview auth_b in
+       length_aux3 auth_b (UInt64.v auth_num);
+       let auth_u = UV.mk_buffer auth_d Views.up_view128 in
+       let abytes_d = get_downview abytes_b in
+       length_aux3 abytes_b 1;      
+       let abytes_u = UV.mk_buffer abytes_d Views.up_view128 in        
+       let cipher_bytes =
+         if UInt64.v plain_num > (UInt64.v len128x6 + UInt64.v len128_num) * 128/8 then
+           UV.as_seq h1 inout_u
+         else Seq.empty
+       in let auth_in =
+         if UInt64.v auth_bytes > UInt64.v auth_num * 128 / 8 then
+           Seq.append (Seq.append (Seq.append (Seq.append (Seq.append
+             (UV.as_seq h0 auth_u) (UV.as_seq h0 abytes_u))
+             (UV.as_seq h1 out128x6_u))
+             (UV.as_seq h1 out128_u))
+             cipher_bytes)
+             (Seq.create 1 length_quad)
+         else
+           Seq.append (Seq.append (Seq.append (Seq.append
+             (UV.as_seq h0 auth_u) (UV.as_seq h1 out128x6_u))
+             (UV.as_seq h1 out128_u))
+             cipher_bytes)
+             (Seq.create 1 length_quad)
+       in
+       DV.length_eq (get_downview tag_b);
+       low_buffer_read TUInt8 TUInt128 h1 tag_b 0 ==
+         gctr_encrypt_block ctr_BE_1 (ghash_LE h auth_in) AES_128 (Ghost.reveal key) 0
+         )
+         ))
     )
